imports Lemma by Andres, begins proof

bedrock2/src/bedrock2Examples/mulhuu.v
@@ -4,6 +4,7 @@ Require Import bedrock2.NotationsCustomEntry.
 Require Import coqutil.Macros.ident_to_string.
 From bedrock2 Require Import WeakestPrecondition ProgramLogic BasicC64Semantics.
 Require Import bedrock2.ZnWords.
+Require Import Lia ZArith.
 
 Import Syntax BinInt String List.ListNotations.
 Import coqutil.Word.Interface.
@@ -16,8 +17,8 @@ Local Notation "x += e" := (cmd.set (ident_to_string! x) (expr.op bopname.add (i
 
 (* Return the high word of the integer multiplication a * b. *)
 Definition mulhuu :=
-  func! (a, b) ~> r2W {
-      W = $4; (* TODO: translate sizeof(uintptr_t)? *)
+  func! (a, b) ~> (r2W, r0) {
+      W = $32;
       M = $1 << W - $1;
       lh = (a & M) * (b >> W);
       hl = (a >> W) * (b & M);
@@ -36,10 +37,75 @@ Definition mulhuu :=
 
 (* mulhuu's functional spec, as commented above. Memory and trace are
    unchanged. *)
-Local Instance spec_of_add_with_carry : spec_of "add_with_carry" :=
-  fnspec! "mulhuu" a b ~> r2W,
+Local Instance spec_of_mulhuu : spec_of "mulhuu" :=
+  fnspec! "mulhuu" a b ~> r2W r0,
     { requires t m := True;
       ensures T M :=
         M = m /\ T = t /\
-          word.unsigned r2W = (word.unsigned a * word.unsigned b) / 2^64
+          2^64 * word.unsigned r2W + word.unsigned r0 =
+            (word.unsigned a * word.unsigned b)
     }.
+
+Ltac cleardisj :=
+  repeat match goal with
+  | H : _ -> _ |- _ => clear H
+  | H : _ \/ _ |- _ => clear H
+  end.
+Ltac cleanby tac :=
+  repeat lazymatch goal with
+  | H : ?A -> ?B |- _ =>
+      specialize (H ltac:(tac))
+      || (assert (not A) as _ by (clear H; tac); clear H)
+      || revert H
+  | H : ?B |- _ =>
+      (assert B as _ by (clear H; tac); clear H)
+      || revert H
+  end; intros; subst.
+Ltac divby tac :=
+  repeat lazymatch goal with
+    H : 0 <= ?m * ?q + _ < ?m*?m |- _ =>
+        try assert (0 <= q < m) by tac; revert H
+  end; intros.
+
+(* a * b can be decomposed into sums of products of low and high-order
+ * bits of a and b. *)
+Lemma mult_half_words :
+  forall
+    m M (Hm : 1 < m < M) (HM : M = m*m)
+    (* (HH : m = 2^32) *)
+    a (Ha : 0 <= a < M)
+    b (Hb : 0 <= b < M)
+    ll (Hll : ll = (a mod m) * (b mod m))
+    hl (Hhl : hl = (a/m) * (b mod m))
+    lh (Hlh : lh = (a mod m) * (b/m))
+    hh (Hll : hh = (a/m) * (b/m))
+    tm (Htm : tm = (ll/m) + (hl mod m) + lh)
+    rh (Hrh : rh = (hl/m) + (tm/m) + hh)
+    rl (Hrl : rl = (tm * m mod M) + (ll mod m)),
+    rh = a * b / M /\
+    rl = a * b mod M.
+Proof.
+  intros.
+  subst M.
+  rewrite Z.mul_mod_distr_r in Hrl by (cleardisj; lia).
+  (* needed for last nia without HH *)
+  Time Z.div_mod_to_equations.
+  Time cleanby ltac:(cleardisj; lia).
+  Fail progress cleanby ltac:(cleardisj; nia).
+  Time progress divby ltac:(cleardisj; lia).
+  Time progress divby ltac:(cleardisj; nia).
+  (* Time Fail nia. (* 9s *) *)
+  match goal with |- ?A /\ _ => assert A; try split; trivial end.
+  (* TODO: these fail with "Expected a single focused goal but 2..."
+  using Coq 8.17.0. *)
+  { nia. }
+  { nia. }
+Qed.
+
+(* Wrapper for `mult_half_words` *)
+(* Lemma mult_half_words' *)
+
+Lemma mulhuu_ok : program_logic_goal_for_function! mulhuu.
+Proof.
+  repeat straightline.
+  Admitted.
